Experimentation w/ pretty printing and more WIP on proof

benchmarks/run_wasm_external_pp.js
@@ -1,0 +1,85 @@
+const fs = require('fs');
+
+var args = process.argv.slice(2);
+
+if (args.length == 0) { process.exit(1); }
+
+binary_path = args[0];
+
+var pp_function;
+
+if (args.length > 1) {
+    if (args[1] == "constructor") { pp_function = '$pretty_print_constructor' }
+    else if (args[1] == "i63") { pp_function = '$pretty_print_i63' }
+}
+
+function write_int (value) {
+    process.stdout.write(value.toString())
+}
+
+function write_char (value) {
+    var chr = String.fromCharCode(value);
+    process.stdout.write(chr);
+}
+
+const print_list = (val, dataView, print_elem) => {
+
+    if (val & 1) { process.stdout.write("nil"); }
+    else {
+	process.stdout.write("(cons ");
+
+	const head = dataView.getInt32(val+4, true);
+
+	print_elem(head, dataView);
+
+	process.stdout.write(" ");
+
+	const tail = dataView.getInt32(val+8, true);
+
+	print_list(tail, dataView, print_elem);
+
+	process.stdout.write(")");
+    }
+}
+
+const print_i63 = (ptr, dataView) => {
+
+    const val = dataView.getBigUint64(ptr, true);
+
+    process.stdout.write(val.toString());
+}
+
+let importObject = {
+    env: {
+        $write_char: write_char,
+        $write_int: write_int,
+    }
+};
+
+(async () => {
+    try {
+	const bytes = fs.readFileSync(binary_path);
+
+	const obj = await WebAssembly.instantiate(
+	    new Uint8Array (bytes), importObject
+	);
+
+	obj.instance.exports.$main_function();
+
+	if (obj.instance.exports.result_out_of_mem.value == 1) {
+            console.log("Ran out of memory.");
+            process.exit(1);
+	} else {
+            const res_value = obj.instance.exports.result.value;
+	    const memory = obj.instance.exports.memory;
+	    const dataView = new DataView(memory.buffer);
+
+	    // print_list(res_value, dataView, print_i63);
+	    print_i63(res_value, dataView);
+
+	    process.stdout.write("\n");
+	}
+    } catch (error) {
+	console.log(error);
+	process.exit(1);
+    }})();
